Dafny test

codegen/smithy-dafny-codegen-test/src/test/java/software/amazon/polymorph/smithyjava/JavaTestModels.java
@@ -40,7 +40,6 @@ class JavaTestModels extends TestModelTest {
     DISABLED_TESTS.add("Union");
     DISABLED_TESTS.add("aws-sdks/kms-lite");
     DISABLED_TESTS.add("aws-sdks/sqs");
-    DISABLED_TESTS.add("aws-sdks/sqs-via-cli");
   }
 
   @ParameterizedTest
