examples/tutorial/SQSExtendedClient/test/SQSExtendedClientImplTest.dfy
@@ -4,16 +4,74 @@ include "../src/Index.dfy"
 
 module {:options "--function-syntax:4"} SQSExtendedClientImplTest {
 
+    import Com.Amazonaws.SQS
+    import ComAmazonawsSqsTypes
     import SQSExtended
     import opened PolymorphTutorialSqsextendedTypes
     import opened Wrappers
 
-    method {:test} TestClient(){
-        // var client :- expect SQSExtendedClient.SQSExtendedClient();
+    method {:test} TestClient() {
+        var sqsClient :- expect SQS.SQSClient();
+        var extendedClient :- expect SQSExtended.SQSExtended(
+            SQSExtendedClientConfig(sqsClient := sqsClient)
+        );
 
         expect false, "...that you'll write actual tests using the client here :)";
         // TestSomeOperation1(client);
         // TestSomeOperation2(client);
         // ...
+    }
+
+    method TestHandleMessages(client: SQSExtended.SQSExtendedClient)
+        requires client.ValidState()
+        modifies client.Modifies
+     {
+        var receiveMessagesRequest := ComAmazonawsSqsTypes.ReceiveMessageRequest(
+            QueueUrl := "foo"
+        );
+        var handler := new MyMessageHandler();
+        var result := client.HandleMessages(PolymorphTutorialSqsextendedTypes.HandleMessagesInput(
+            receiveRequest := receiveMessagesRequest,
+            handler := handler
+        )); 
+    }
+
+
+    class MyMessageHandler extends PolymorphTutorialSqsextendedTypes.IMessageHandler {
+        constructor() 
+            ensures ValidState()
+            ensures fresh(History)
+            ensures fresh(Modifies)
+        {
+            History := new IMessageHandlerCallHistory();
+            Modifies := {History};
+        }
+
+        ghost predicate ValidState()
+            ensures ValidState() ==> History in Modifies 
+        {
+            History in Modifies 
+        }
+
+        ghost predicate HandleMessageEnsuresPublicly(input: HandleMessageInput , output: Result<(), Error>)
+        {
+            true
+        }
+
+        method HandleMessage' ( input: HandleMessageInput )
+            returns (output: Result<(), Error>)
+            requires
+                && ValidState()
+            modifies Modifies - {History}
+            // Dafny will skip type parameters when generating a default decreases clause.
+            decreases Modifies - {History}
+            ensures
+                && ValidState()
+            ensures HandleMessageEnsuresPublicly(input, output)
+            ensures unchanged(History)
+        {
+            print "Got a message: ", input.message.Body;
+            return Success(());
+        }
     }
 }
